Quotify/Theorem.lean
@@ -5,11 +5,11 @@ import Quotify.Mathlib
 
 open Lean Meta
 
-namespace Quotify
+namespace Quotify.Theorem
 
 -- **TODO** Add some flexibility to the order of parameters in theorem kinds.
 
-public inductive Theorem.Kind where
+public inductive Kind where
   /-- Theorems of the form `∀ …, ∀ a b, (a ≈ b) → f a = f b`. -/
   | lift
   /-- Theorems of the form `∀ …, ∀ a₁ b₁ a₂ b₂, (a₁ ≈ a₂) → (b₁ ≈ b₂) → f a₁ b₁ = f a₂ b₂`. -/
@@ -20,24 +20,64 @@ public inductive Theorem.Kind where
   | map₂
   deriving BEq, Hashable, Inhabited
 
-public instance Theorem.Kind.instToString : ToString Theorem.Kind where
+public instance Kind.instToString : ToString Theorem.Kind where
   toString
     | .lift  => "lift"
     | .lift₂ => "lift₂"
     | .map   => "map"
     | .map₂  => "map₂"
 
-public structure Theorem where
-  declName       : Name
-  numParams      : Nat
-  numLevelParams : Nat
+/--
+Creates a list of `n` fresh mvars of the given `type`, where `n` is the number of arguments expected
+by the function in a theorem of the given `Kind`. For example, for `Kind.map` this is `1` and for
+`Kind.map₂` it is `2`.
+-/
+public def Kind.freshArgMVars (type : Expr) : Kind → MetaM (Array Expr)
+  | .map  | .lift  => return #[← mkFreshExprMVar type]
+  | .map₂ | .lift₂ => return #[← mkFreshExprMVar type, ← mkFreshExprMVar type]
+
+public structure Function where
+  /-- An (abstraction over) the target function (called `f` in the documentation comments on
+     `Theorem.Kind`) of the given theorem. Thus `fn` has the form `λ a₁ … aₙ, f a₁ … aₙ` where
+     `a₁ … aₙ` are the arguments parameterizing the theorem (the `…` in the documentation comments
+     on `Theorem.Kind`). -/
+  fn : Expr
+  /-- The number of arguments parameterizing `fn`. For `λ a₁ … aₙ, f a₁ … aₙ` where we have
+      `numParams = n`. If `f a₁ … aₙ` is itself a `λ` with two arguments, we get
+      `λ a₁ … aₙ lhs rhs, … lhs rhs`, but still have `numParams = n`. -/
+  numParams : Nat
   deriving BEq, Inhabited
 
-namespace Theorem
+public structure _root_.Quotify.Theorem extends Function where
+  declName : Name
+  /-- The names of the level parameters over the theorem (and thus, potentially `fn`) is abstracted.
+      Note, this field is unrelated to `numParams`. -/
+  levelParams : List Name
+  deriving BEq, Inhabited
 
-def isMap₂ (mvars : Array Expr) (lhs rhs : Expr) (binRel : BinRel) : MetaM (Option Nat) := do
-  let numTargets := 6
-  let [a₁, a₂, aEquiv, b₁, b₂, bEquiv] := mvars[(mvars.size - numTargets)...mvars.size].toList | return none
+-- **TODO** Ensure that `fᵢ` is not itself a parameter?
+def map? (mvars : Array Expr) (lhs rhs : Expr) (binRel : BinRel) : MetaM (Option Theorem.Function) := do
+  let targetsStartIdx := mvars.size - 3
+  let [a, b, equiv] := mvars[targetsStartIdx...mvars.size].toList | return none
+  let .app f₁ a' := lhs | return none
+  let .app f₂ b' := rhs | return none
+  unless f₁ == f₂ && a == a' && b == b' do return none
+  let equivType ← inferType equiv
+  let .success equivRel _ ← BinRel.fromFullyApplied equivType | return none
+  -- **TODO** This need not be the same equivalence relation.
+  unless binRel == equivRel do return none
+  let params := mvars[0...targetsStartIdx]
+  let numParams := params.size
+  -- This is a low-effort check that the theorem's leading parameters are (at least the same number
+  -- as) those abstracting the equivalence relation.
+  unless numParams == equivRel.numParams do return none
+  let fn ← mkLambdaFVars params f₁
+  return some { fn, numParams }
+
+-- **TODO** Ensure that `fᵢ` is not itself a parameter?
+def map₂? (mvars : Array Expr) (lhs rhs : Expr) (binRel : BinRel) : MetaM (Option Theorem.Function) := do
+  let targetsStartIdx := mvars.size - 6
+  let [a₁, a₂, aEquiv, b₁, b₂, bEquiv] := mvars[targetsStartIdx...mvars.size].toList | return none
   let .app (.app f₁ a₁') b₁' := lhs | return none
   let .app (.app f₂ a₂') b₂' := rhs | return none
   unless f₁ == f₂ && a₁ == a₁' && a₂ == a₂' && b₁ == b₁' && b₂ == b₂' do return none
@@ -45,27 +85,15 @@ def isMap₂ (mvars : Array Expr) (lhs rhs : Expr) (binRel : BinRel) : MetaM (Op
   let bEquivType ← inferType bEquiv
   let .success aEquivRel _ ← BinRel.fromFullyApplied aEquivType | return none
   let .success bEquivRel _ ← BinRel.fromFullyApplied bEquivType | return none
+  -- **TODO** This need not be the same equivalence relation.
   unless binRel == aEquivRel && aEquivRel == bEquivRel do return none
-  let numParams := mvars.size - numTargets
+  let params := mvars[0...targetsStartIdx]
+  let numParams := params.size
   -- This is a low-effort check that the theorem's leading parameters are (at least the same number
   -- as) those abstracting the equivalence relation.
   unless numParams == aEquivRel.numParams do return none
-  return numParams
-
-def isMap (mvars : Array Expr) (lhs rhs : Expr) (binRel : BinRel) : MetaM (Option Nat) := do
-  let numTargets := 3
-  let [a, b, equiv] := mvars[(mvars.size - numTargets)...mvars.size].toList | return none
-  let .app f₁ a' := lhs | return none
-  let .app f₂ b' := rhs | return none
-  unless f₁ == f₂ && a == a' && b == b' do return none
-  let equivType ← inferType equiv
-  let .success equivRel _ ← BinRel.fromFullyApplied equivType | return none
-  unless binRel == equivRel do return none
-  let numParams := mvars.size - numTargets
-  -- This is a low-effort check that the theorem's leading parameters are (at least the same number
-  -- as) those abstracting the equivalence relation.
-  unless numParams == equivRel.numParams do return none
-  return numParams
+  let fn ← mkLambdaFVars params f₁
+  return some { fn, numParams }
 
 public def forThm? (thmInfo : TheoremVal) : MetaM <| Option (Theorem × Kind × BinRel) := do
   let thmType := thmInfo.type.cleanupAnnotations
@@ -73,42 +101,75 @@ public def forThm? (thmInfo : TheoremVal) : MetaM <| Option (Theorem × Kind × 
   let #[lhs, rhs] := body.getBoundedAppArgs 2 | return none
   let rel := body.stripArgsN 2
   let .success binRel _ ← BinRel.fromExpr rel | return none
-  if let some numParams ← isMap mvars lhs rhs binRel then
-    let thm := { declName := thmInfo.name, numParams, numLevelParams := thmInfo.levelParams.length }
+  if let some f ← map? mvars lhs rhs binRel then
+    let thm := { f with declName := thmInfo.name, levelParams := thmInfo.levelParams }
     return some (thm, .map, binRel)
-  else if let some numParams ← isMap₂ mvars lhs rhs binRel then
-    let thm := { declName := thmInfo.name, numParams, numLevelParams := thmInfo.levelParams.length }
+  else if let some f ← map₂? mvars lhs rhs binRel then
+    let thm := { f with declName := thmInfo.name, levelParams := thmInfo.levelParams }
     return some (thm, .map₂, binRel)
   else
     return none
 
-public structure Simp where
-  declName : Name
-  expr     : Expr
+/--
+Given `thm.fn` of the form `λ a₁ … aₙ, f a₁ … aₙ`, instantiates the binders with mvars and returns
+`(params : Array Expr) × (lmvars : List Level) × (fn : Expr)` with `params` being the mvars for
+`a₁ … aₙ`, `lmvars` being the the level mvars instantiated for `thm.levelParams`, and `fn` being
+instantiated to `f params`.
+-/
+def metaTelescope (thm : Theorem) : MetaM (Array Expr × List Level × Expr) := do
+  -- It's important that we instantiate the level params with level mvars *before* we telescope, as
+  -- otherwise the types of the created (expr) mvars still refer to the level params.
+  let freshLMVars     ← mkFreshLevelMVars thm.levelParams.length
+  let fn             := thm.fn.instantiateLevelParams thm.levelParams freshLMVars
+  let (params, _, fn) ← lambdaMetaTelescope fn (maxMVars? := thm.numParams)
+  return (params, freshLMVars, fn)
 
-def mkFreshExprMVars (num : Nat) : MetaM (Array Expr) :=
-  num.foldM (init := #[]) fun _ _ acc => return acc.push (← mkFreshExprMVar none)
+structure Match where
+  params : Array Expr
+  levels : List Level
 
-def mvarApplied (thm : Theorem) : MetaM Expr := do
-  let lmvars ← mkFreshLevelMVars thm.numLevelParams
-  let mvars ← mkFreshExprMVars thm.numParams
-  return mkAppN (.const thm.declName lmvars) mvars
+/--
+Tries to match a given `target` against a `thm`'s `fn` up to definitional equality. If the match
+succeeds a substitution (a `Match`) for `target`'s parameters is returned.
 
-public def simp (thm : Theorem) : Theorem.Kind → MetaM Theorem.Simp
+Matching is asymmetric in that the `thm.fn` must be more abstract than the `target`. For example,
+`thm.fn = λ α, @List.reverse α` will match `target = @List.reverse Nat`, but not the other way
+around.
+-/
+def match? (thm : Theorem) (target : Expr) : MetaM (Option Match) := do
+  -- We bump the mvar context depth so that only `thm.fn`s (abstracted) parameters can be matched
+  -- but not the other way around. For example, this means that `@List.reverse ?α` can be matched
+  -- against `@List.reverse Nat`, but not vice versa.
+  withNewMCtxDepth do
+    let (params, lmvars, fn) ← thm.metaTelescope
+    if ← isDefEq fn target then
+      let params ← params.mapM instantiateMVars
+      let levels ← lmvars.mapM instantiateLevelMVars
+      return some { params, levels }
+    else
+      return none
+
+/--
+Checks that the given `thm.fn` matches the given `target`, and if so produces a proof for `thm`
+specialized to the `target`. For example, if `thm.fn` is
+`∀ α a b, a ≈ b → List.reverse a ≈ List.reverse b` and `target` is `@List.reverse Nat`, then
+`specialize?` produces a proof of `∀ a b, a ≈ b → @List.reverse Nat a ≈ @List.reverse Nat b`.
+
+Note that for theorems where `fn` is not parameterized, this function amounts to just checking that
+the `thm` is applicable to the `target` and returning the "default" proof.
+-/
+def specialize? (thm : Theorem) (target : Expr) : MetaM (Option Expr) := do
+  let some m ← thm.match? target | return none
+  return mkAppN (.const thm.declName m.levels) m.params
+
+-- **DOC**
+public def mkPush? (thm : Theorem) (app : Expr) (setoid : Expr) : Theorem.Kind → MetaM (Option Expr)
   | .map => do
-    let quotientMapMk ← mkConstWithFreshMVarLevels ``Quotient.map_mk
-    let mvars ← mkFreshExprMVars 5
-    let compatThm ← thm.mvarApplied
-    let args := mvars.push compatThm
-    let expr := mkAppN quotientMapMk args
-    return { declName := thm.declName, expr }
-  | .map₂ => do
-    let quotientMap₂Mk ← mkConstWithFreshMVarLevels ``Quotient.map₂_mk
-    let mvars ← mkFreshExprMVars 7
-    let compatThm ← thm.mvarApplied
-    let args := mvars.push compatThm
-    let expr := mkAppN quotientMap₂Mk args
-    return { declName := thm.declName, expr }
+    let .app fn arg := app | return none
+    let some h ← thm.specialize? fn | return none
+    let argType ← inferType arg
+    let lvl ← getLevel argType
+    let eq := mkApp7 (.const ``Quotient.map_mk [lvl, lvl]) argType argType setoid setoid fn h arg
+    mkEqSymm eq
   | _ =>
-    -- **TODO**
-    return { declName := .anonymous, expr := mkNatLit 0 }
+    return none -- **TODO**
