Tests/PushQuotients.lean
@@ -1,24 +1,34 @@
 import Quotify.Tactic
 import Quotify.Command
--- import Quotify.Unexpanders
+import Quotify.Unexpanders
 
 @[quotify]
 theorem t (l₁ l₂ : List α) (h : l₁ ≈ l₂) : l₁.reverse ≈ l₂.reverse := sorry
 
 attribute [quotify] List.isSetoid
 
+open Lean Meta Elab Term Simp
+
+def pushT : Simproc := fun e => do
+  let_expr Quotient.mk listType setoid app := e | return .continue
+  let .app fn l := app | return .continue
+
+  let lvl ← getLevel listType
+  let thm := mkApp (.const ``t [lvl]) listType
+
+  let prf := mkApp7 (.const ``Quotient.map_mk [lvl, lvl]) listType listType setoid setoid fn thm l
+  let prf ← mkEqSymm prf
+  let_expr Eq _ _ pushed := ← inferType prf | return .continue
+  return .visit { expr := pushed, proof? := prf }
+
+#eval do
+  -- following elabSimprocKeys
+  let pattern : Expr ← elabTerm (← `(@Quotient.mk _ _ _)) none
+  Term.synthesizeSyntheticMVars
+  let keys ← withSimpGlobalConfig <| DiscrTree.mkPath pattern
+  registerSimproc ``pushT keys
+
 example (l₁ l₂ : List α) (h : l₁.reverse ≈ l₂.reverse) : l₁ ≈ l₂ := by
   quotify
-  -- **TODO** I think the problem is that the setoid is not being matched. Can we avoid this by
-  --          using the original setoid matched for the relation when constructing the
-  --          iffQuotientEq theorem?
-  --
-  --          More generally, the `Quotient.*` theorems rewrite the compatability theorems to be
-  --          stated specifically in terms of `≈`. So if we change the `≈` in `t` to `List.Perm`, we
-  --          get an application mismatch when constructing the term `Quotient.map_mk ...` below.
-  --          Should we require `≈` in `quotify` theorems too, or just construct an equivalent
-  --          theorem that uses `≈` on the fly, when necessary?
-
-  simp only [← @Quotient.map_mk _ _ _ _ _ (@t _)] at h
-  rw [← Quotient.map_mk _ t] at h
-  erw [← Quotient.map_mk _ t] at h
+  simp only [↓pushT] at *
+  sorry
