Quotify.lean
@@ -1,1 +1,9 @@
-import Quotify.Translate
+import Quotify.Attribute
+import Quotify.Batteries
+import Quotify.BinRel
+import Quotify.Command
+import Quotify.Mathlib
+import Quotify.Setoid
+import Quotify.Tactic
+import Quotify.Theorem
+import Quotify.Unexpanders
