Quotify/Tactic.lean
@@ -10,6 +10,10 @@ meta def Lean.LocalContext.getVisibleFVarIds (lctx : LocalContext) : Array FVarI
 
 namespace Quotify
 
+-- **TODO** Swapping the relation need not be a separate step from pushing the quotients. We can perform
+--          them all in a single simproc. Namely, once the swap-relation simproc applies it calls the
+--          sub-simproc for pushing the quotients.
+
 /--
 Replaces all occurrences of `binRel` in the goal and local context with the corresponding quotient
 equality relation, proven equal by `iffQuotEq`.
@@ -27,7 +31,13 @@ meta def swapRelation (binRel : BinRel) (iffQuotEq : Expr) : TacticM Unit := do
                     quotients."
     replaceMainGoal [goal]
 
-meta def pushQuotients (binRel : BinRel) : TacticM Unit := do
+meta def pushQuotients (binRel : BinRel) (setoid : Extension.Setoid) : TacticM Unit := do
+  -- The given `binRel` and `setoid` are derived from the proof goal and should therefore not be
+  -- abstract over any parameters.
+  let lvl ← getLevel binRel.argType
+  let setoid := mkApp3 (.const ``_root_.Setoid.mk [lvl]) binRel.argType binRel.expr setoid.equiv.proof
+  return
+  /-
   let goal ← getMainGoal
   goal.withContext do
     let thms ← extension.getMatchingTheorems binRel
@@ -42,6 +52,7 @@ meta def pushQuotients (binRel : BinRel) : TacticM Unit := do
     let (some (_, goal), _) ← simpGoal goal simpCtx (fvarIdsToSimp := fvarIdsToSimp)
       | throwError "`quotify` failed to push quotients."
     replaceMainGoal [goal]
+  -/
 
 elab tk:"quotify" : tactic =>
   withRef tk <| withMainContext do
@@ -55,4 +66,4 @@ elab tk:"quotify" : tactic =>
                      for the relation {indentExpr binRel.expr}"
     let iffQuotEq ← binRel.mkIffQuotientEq setoid.equiv.proof
     swapRelation binRel iffQuotEq
-    pushQuotients binRel
+    pushQuotients binRel setoid
