Tests/Deprecated/Monoid_norm/Monoid_norm(setoidRw).lean
@@ -1,0 +1,101 @@
+import Quotify.Translate
+import Quotify.Signature
+import Quotify.Attribute
+
+-- From: https://cs.ioc.ee/ewscs/2009/dybjer/mainPalmse-revised.pdf
+
+inductive Exp (α : Type)
+| app : Exp α → Exp α → Exp α
+| id  : Exp α
+| elem : α → Exp α
+
+
+inductive R : {α : Type} → (Exp α) → (Exp α) → Prop
+| assoc {e e' e'' : Exp α} : R ((e.app e').app e'') (e.app (e'.app e''))
+| id_left {e  : Exp α}     : R ((Exp.id).app e) (e)
+| id_right {e : Exp α}     : R (e.app Exp.id) (e)
+| refl     {e : Exp α}     : R (e) (e)
+| symm      {e e' : Exp α} : R (e) (e') → R (e') (e)
+| trans {e e' e'' : Exp α} : R (e) (e') → R (e') (e'') → R (e) (e'')
+| app {a b c d : Exp α}    : R (a) (b) → R (c) (d) → R (a.app c) (b.app d)
+
+
+-- Setoid instance here:
+instance R_Setoid : Setoid (Exp α) :=
+  { r := @R α
+    iseqv :=
+      { refl := λ _ => R.refl
+        symm := R.symm
+        trans := R.trans
+      }
+  }
+
+def app_sig (α : Type) : (Respectful R <| Respectful R R) (@Exp.app α) (@Exp.app α) :=
+  fun x y a x_2 y_2 a_1 => R.app a a_1
+
+def eval : (Exp α) → (Exp α → Exp α)
+  | Exp.app a b => (λ e => eval a (eval b e))
+  | Exp.id      => id
+  | Exp.elem x  => (λ e => (Exp.elem x).app e)
+
+
+set_option pp.all true in
+-- ∀ b, a.app b ~ [[a]]b
+theorem eval_lemma1 {α : Type} (a : Exp α) : ∀ b, R (a.app b) ((eval a) b) := by
+  induction a
+
+  case app c d c_ih d_ih =>
+    unfold eval
+    intro b
+    specialize d_ih b
+    specialize c_ih (eval d b)
+
+    have R.assoc := @R.assoc
+
+    translateF [⟨Exp.app, app_sig⟩]
+    -- (c ⬝ d) ⬝ b ~ c ⬝ (d ⬝ b) ~ c ⬝ (eval d b) ~ eval c (eval d b)
+    rw [R.assoc, d_ih, c_ih]
+
+  case id =>
+    intro b
+    exact R.id_left
+
+  case elem =>
+    intro b
+    exact R.refl
+
+
+@[quotify]
+theorem eval_sig : (α : Type) → (Respectful R Eq) (@eval α) (@eval α) := by
+  sorry
+
+
+def reify (f : Exp α → Exp α) : (Exp α) := f Exp.id
+
+def nbe (e : Exp α) : Exp α := reify (eval e)
+
+-- Shows decidability of e ~ e'
+theorem correctness (e e' : Exp α) : (R (e) (e')) ↔ (nbe e = nbe e') :=
+by
+  apply Iff.intro
+  · intro h
+    induction h
+    any_goals
+      grind
+    case mp.app a b c d a_r_b c_r_d _ _ =>
+      -- clear * - a_r_b c_r_d
+      unfold nbe reify
+      translateF
+                [⟨Exp.app, app_sig⟩,
+                 ⟨eval, eval_sig⟩]
+      grind
+
+  · unfold nbe reify
+    intro h0
+    -- Translate "R a b" to "⟦a⟧ = ⟦b⟧"
+    have R.id_right := @R.id_right
+    have eval_lemma1:= @eval_lemma1
+    translateF []
+    -- e ~ e ⬝ id ~ nbe e = nbe e' ~ e' ⬝ id ~ e'
+    rw [← R.id_right, eval_lemma1 e Exp.id, h0,
+                    ← eval_lemma1 e' Exp.id, R.id_right]
