Tests/Deprecated/Monoid_norm/Monoid_norm.lean
@@ -1,0 +1,132 @@
+import Quotify.Translate
+-- From: https://cs.ioc.ee/ewscs/2009/dybjer/mainPalmse-revised.pdf
+
+inductive Exp (α : Type)
+| app : Exp α → Exp α → Exp α
+| id  : Exp α
+| elem : α → Exp α
+
+
+inductive R : (Exp α) → (Exp α) → Prop
+| assoc {e e' e'' : Exp α} : R ((e.app e').app e'') (e.app (e'.app e''))
+| id_left {e  : Exp α}     : R ((Exp.id).app e) (e)
+| id_right {e : Exp α}     : R (e.app Exp.id) (e)
+| refl     {e : Exp α}     : R (e) (e)
+| symm      {e e' : Exp α}  : R (e) (e') → R (e') (e)
+| trans {e e' e'' : Exp α} : R (e) (e') → R (e') (e'') → R (e) (e'')
+| app {a b c d : Exp α}    : R (a) (b) → R (c) (d) → R (a.app c) (b.app d)
+
+
+def eval : (Exp α) → (Exp α → Exp α)
+  | Exp.app a b => (λ e => eval a (eval b e))
+  | Exp.id      => id
+  | Exp.elem x  => (λ e => (Exp.elem x).app e)
+
+-- ∀ b, a.app b ~ [[a]]b
+theorem eval_lemma1 (a : Exp α) : ∀ b, R (a.app b) ((eval a) b) := by
+  induction a
+  case app c d c_ih d_ih =>
+    intro b
+    specialize d_ih b
+    specialize c_ih (eval d b)
+    -- R-rewriting here
+    have h0 : R ((c.app d).app b) (c.app (d.app b)) := R.assoc
+    refine (R.trans h0 ?_)
+    clear h0
+    have h0 : R (c.app (d.app b)) (c.app (eval d b)) := R.app (R.refl) (d_ih)
+    refine (R.trans h0 ?_)
+    clear h0
+    exact c_ih
+
+  case id =>
+    intro b
+    exact R.id_left
+
+  case elem =>
+    intro b
+    exact R.refl
+
+-- a ~ b  → ∀ c, [[a]]c = [[b]]c
+theorem eval_lemma2 {a b : Exp α} (h : R a b) : ∀ c : Exp α, (eval a) c = (eval b) c := by
+  induction h
+
+  any_goals
+    intros; grind
+
+  case app a b c d _ _ ab_ih cd_ih =>
+    -- clear  - ab_ih cd_ih
+    intro e
+    specialize cd_ih e
+    specialize ab_ih ((eval d) e)
+    simp only [eval]
+    rw [cd_ih]
+    rw [ab_ih]
+  all_goals sorry
+
+
+def reify (f : Exp α → Exp α) : (Exp α) := f Exp.id
+
+def nbe (e : Exp α) : Exp α := reify (eval e)
+
+-- Shows decidability of e ~ e'
+theorem correctness (e e' : Exp α) : (R (e) (e')) ↔ (nbe e = nbe e') := by
+  apply Iff.intro
+  · intro h
+    induction h
+    any_goals
+      aesop
+    case mp.app a b c d a_r_b c_r_d _ _ =>
+      clear * - a_r_b c_r_d
+      apply eval_lemma2 ?_ Exp.id
+      -- R-rewriting here
+      exact R.app a_r_b c_r_d
+
+  · unfold nbe reify
+    intro h0
+    -- R-rewriting here
+    have h1 : R (e) (e.app Exp.id) := (R.symm R.id_right)
+    refine (R.trans h1 ?_)
+    clear h1
+    have h1 : R (e.app Exp.id) ((eval e) Exp.id) := eval_lemma1 e Exp.id
+    refine (R.trans h1 ?_)
+    clear h1
+    rewrite [h0]
+    clear h0
+    have h0 : R ((eval e') Exp.id) (e'.app Exp.id) := R.symm (eval_lemma1 e' Exp.id)
+    refine (R.trans h0 ?_)
+    clear h0
+    exact R.id_right
+
+
+
+
+-- ((1, 2), ((0, 0), 3)) ~ ((0, 0), (1, (2, (0, 3))))
+def zero := (Exp.id : Exp Nat)
+def one  := Exp.elem 1
+def two  := Exp.elem 2
+def three := Exp.elem 3
+example : R
+          ( (one.app two).app  ((zero.app zero).app three) )
+          ( (zero.app zero).app (one.app (two.app (zero.app three)))) :=
+  by
+  have h0 : R (zero.app zero)  zero := R.id_left
+  have h1 : R ((zero.app zero).app three) (zero.app three) := R.app h0 R.refl
+-- ((1, 2), ((0, 0), 3)) ~ ((1, 2), (0, 3))
+  have h2 : R ((one.app two).app ((zero.app zero).app three))
+                  ((one.app two).app (zero.app three)) := R.app R.refl h1
+-- ((1, 2), (0, 3)) ~ (1, (2, (0, 3))
+  have h3 : R ((one.app two).app (zero.app three))
+                  (one.app (two.app (zero.app three))) := R.assoc
+  have h4 : R zero (zero.app zero) := R.symm h0
+-- (1, (2, (0, 3)) ~ (0, (1, (2, (0, 3)))
+  have h5 : R (one.app (two.app (zero.app three)))
+                  (zero.app (one.app (two.app (zero.app three)))) := R.symm R.id_left
+-- (0, (1, (2, (0, 3))) ~ ((0, 0), (1, (2, (0, 3)))
+  have h6 : R (zero.app (one.app (two.app (zero.app three))))
+                  ((zero.app zero).app (one.app (two.app (zero.app three)))) := R.app h4 R.refl
+  clear h0 h1 h4
+  apply R.trans h2
+  apply R.trans h3
+  apply R.trans h5
+  apply R.trans h6
+  exact R.refl
