Tests/Deprecated/Nat_mod/Nat_mod.lean
@@ -1,0 +1,35 @@
+import Quotify.Translate
+
+def R : Nat → Nat → Nat → Prop := fun n x y => x.mod n = y.mod n
+
+-- Setoid instance here:
+instance R_Setoid (n : Nat) : Setoid Nat where
+  r := R n
+  iseqv := sorry
+
+/-
+def add_sig : (n : Nat) → Signature (Nat.add) ((R n) ⟹ (R n) ⟹ (R n)) :=
+  by
+  sorry
+
+
+def mul_sig :  (n : Nat) → Signature (Nat.mul) ((R n) ⟹ (R n) ⟹ (R n)) :=
+  by sorry
+-/
+
+example (x_R_y : R n x y) : R n (3 * (1 + (7 + x) + 5)) ((1 + 7 + y + 5) * 3) := by
+  -- TODO: The setoid approach already does not make sense here. Over which type is the setoid?
+  --       `Nat`?
+  translateF
+    [⟨Nat.add, add_sig⟩,
+     ⟨Nat.mul, mul_sig⟩]
+  rw [x_R_y]
+  translateB
+    [⟨Nat.add, add_sig⟩,
+     ⟨Nat.mul, mul_sig⟩]
+
+  suffices eq : (Nat.mul 3 ((Nat.add 1 (Nat.add 7 y)).add 5)) = ((((Nat.add 1 7).add y).add 5).mul 3)
+    by
+    rewrite [eq] ; clear eq
+    sorry
+  grind
