Tests/Deprecated/SetEq.lean
@@ -1,0 +1,66 @@
+-- import Quotify.Signature
+-- import Quotify.Translate
+-- import Quotify.Attribute
+import Quotify.Unexpanders
+/-
+From:
+  https://github.com/FWuermse/grw/blob/main/GrwTest/SetEq.lean
+-/
+
+def setEq {α : Type} : List α → List α → Prop :=
+  fun l1 l2 => ∀ x, x ∈ l1 <-> x ∈ l2
+
+instance setEqEquivalence {α : Type} : Equivalence (@setEq α) where
+  refl := fun l1 x => Iff.rfl
+  symm := by
+    intro x y hxy
+    unfold setEq
+    intro a
+    apply Iff.symm
+    exact hxy a
+  trans := by
+    intro x y z hxy hyz
+    unfold setEq at *
+    intro a
+    apply Iff.intro
+    intro hx
+    rw [hxy a] at hx
+    rw [hyz a] at hx
+    assumption
+    intro hy
+    rw [← hyz a] at hy
+    rw [← hxy a] at hy
+    assumption
+
+instance Setoid_List {α : Type} : Setoid (@List α) where
+  r     := fun l1 l2 => ∀ x, x ∈ l1 <-> x ∈ l2
+  iseqv := setEqEquivalence
+
+def addElem {α : Type} (x : α) (l : List α) : List α :=
+  x :: l
+
+
+
+theorem addElem_sig (x : α) : ∀ (a₁ a₂ : List α), a₁ ≈ a₂ → addElem x a₁ ≈ addElem x a₂ := by
+  intro a₁ a₂ heq x
+  simp [addElem]
+  constructor
+  · intro hx
+    cases hx with
+    | inl => left; assumption
+    | inr h' =>
+      right; exact (heq x).mp h'
+  · intro hx
+    cases hx with
+    | inl => left; assumption
+    | inr h' => right; exact (heq x).mpr h'
+
+theorem rewriteExample (h : setEq [1,2,3] [3,2,1]) : setEq (addElem 4 [1,2,3]) (addElem 4 [3,2,1]) := by
+  have e : @setEq Nat = (fun lhs rhs => Quotient.mk Setoid_List lhs = Quotient.mk Setoid_List rhs) := sorry
+  revert h
+  simp only [e]
+  intro h
+  clear e
+  simp only [← Quotient.map_mk _ (addElem_sig _) _]
+  -- --
+  rw [h]
