Tests/PushThms.lean
@@ -1,0 +1,21 @@
+import Quotify.Command
+
+@[quotify]
+theorem t (l₁ l₂ : List α) (h : l₁ ≈ l₂) : l₁.reverse ≈ l₂.reverse := sorry
+
+@[quotify]
+theorem s (l₁ l₂ : List Nat) (h : l₁ ≈ l₂) : l₁.reverse ≈ l₂.reverse := sorry
+
+attribute [quotify] List.isSetoid
+
+/--
+info:
+t: fun {x} => Eq.symm (Quotient.map_mk List.reverse t x)
+s: fun {x} => Eq.symm (Quotient.map_mk List.reverse s x)
+-/
+#guard_msgs in
+#quotify_push @List.Perm Nat
+
+/-- info: t: fun x_0 {x} => Eq.symm (Quotient.map_mk List.reverse t x) -/
+#guard_msgs in
+#quotify_push @List.Perm
